Added TRUE and FALSE constructors to Presence Conditions and some examples of programs.

STLC_SuccNat/Lifted_STLC_SuccNat.v
@@ -1,5 +1,5 @@
 Require Import STLC_SuccNat.
-Require Import String List.
+Require Import String List Maps.
 Import ListNotations.
 
 Open Scope string_scope.
@@ -11,7 +11,9 @@ Inductive PresenceCondition : Type :=
   | PC_Feature : Feature -> PresenceCondition
   | PC_And     : PresenceCondition -> PresenceCondition -> PresenceCondition
   | PC_Or      : PresenceCondition -> PresenceCondition -> PresenceCondition
-  | PC_Not     : PresenceCondition -> PresenceCondition.
+  | PC_Not     : PresenceCondition -> PresenceCondition
+  | PC_True    : PresenceCondition
+  | PC_False   : PresenceCondition.
 
 Declare Custom Entry pc_syntax.
 
@@ -24,6 +26,8 @@ Notation "x '\/' y" := (PC_Or x y)
   (in custom pc_syntax at level 50, left associativity).
 Notation "'~' x" := (PC_Not x)
   (in custom pc_syntax at level 35, right associativity).
+Notation "'TRUE'" := PC_True (in custom pc_syntax at level 0).
+Notation "'FALSE'" := PC_False (in custom pc_syntax at level 0).
 Notation "'(' x ')'" := x
   (in custom pc_syntax, x at level 0).
 Notation "'[[' x ']]'" := x
@@ -34,13 +38,15 @@ Definition FeatureConfig := list Feature.
 
 (* Function that evaluates a Presence Condition given a Feature Configuration *)
 (* Q: Should I do a relational definition of this function?
-      Since it might be easier to prove somethings *)
+      Since it might be easier to prove something *)
 Fixpoint pc_eval (cfg : FeatureConfig) (pc : PresenceCondition) : bool :=
   match pc with
   | PC_Feature f => if in_dec String.string_dec f cfg then true else false
   | PC_And p1 p2 => pc_eval cfg p1 && pc_eval cfg p2
   | PC_Or  p1 p2 => pc_eval cfg p1 || pc_eval cfg p2
   | PC_Not p1   => negb (pc_eval cfg p1)
+  | PC_True => true
+  | PC_False => false
   end.
 
 Definition pc1 := [[ (FEATURE "A") /\ (FEATURE "B") ]].
@@ -52,8 +58,43 @@ Compute pc_eval [] pc2.
 Definition pc3 := [[ (FEATURE "A") /\ ~ (FEATURE "B") \/ (FEATURE "C") ]].
 Compute pc_eval ["A"; "B"; "C"] pc2.
 
+Definition pc4 := [[ TRUE /\ (FEATURE "A") ]].
+Compute pc_eval ["A"] pc4.
 
+Definition pc5 := [[ FALSE /\ (FEATURE "A") ]].
+Compute pc_eval ["A"] pc5.
 
+Definition plustwo := abs "n" Nat (succ (succ (var "n"))).
 
+Example ty_plustwo: has_type empty plustwo (Arrow Nat Nat).
+Proof.
+  apply T_Abs.
+  apply T_Succ. apply T_Succ.
+  apply T_Var. reflexivity.
+Qed.
+
+Example plustwo_3_is_5:
+  step_normal_form_of (STLC_SuccNat.app plustwo (const 3)) (const 5).
+Proof.
+  split.
+  - eapply multi_step.
+    + apply ST_AppAbs. apply v_nat.
+    + eapply multi_step.
+      * simpl. eapply ST_Succ. apply ST_SuccConst.
+      * eapply multi_step.
+        ** apply ST_SuccConst.
+        ** apply multi_refl.
+  - intros [t' Contra]. inversion Contra.
+Qed.
+
+Definition lifted_plustwo := [(abs "n" Nat (succ (succ (var "n"))), [[TRUE]])].
+Check lifted_plustwo.
+
+Definition lifted_n :=
+  [
+   (1, [[FEATURE "A"]]);
+   (2, [[~ (FEATURE "A") /\ (FEATURE "B")]]);
+   (3, [[~ (FEATURE "A") /\ ~ (FEATURE "B")]])
+  ].
 
 (* Lifted Types *)
